Preliminary support for small data area in PowerPC port.
git-svn-id: https://yquem.inria.fr/compcert/svn/compcert/trunk@1163 fca1b0fc-160b-0410-b1d3-a4f43f01ea2e

driver/Clflags.ml
@@ -17,6 +17,7 @@ let linker_options = ref ([]: string list)
 let exe_name = ref "a.out"
 let option_flonglong = ref false
 let option_fmadd = ref false
+let option_fsda = ref false
 let option_dclight = ref false
 let option_dasm = ref false
 let option_E = ref false
